@prefix owl: <http://www.w3.org/2002/07/owl#> .
@prefix xsd: <http://www.w3.org/2001/XMLSchema#> .
@prefix dct: <http://purl.org/dc/terms/> .
@prefix rdf: <http://www.w3.org/1999/02/22-rdf-syntax-ns#> .
@prefix rdfs: <http://www.w3.org/2000/01/rdf-schema#> .
@prefix skos: <http://www.w3.org/2004/02/skos/core#> .
@prefix unms: <http://unontologies.s3-website-us-east-1.amazonaws.com/unms#> .
@prefix undoc: <http://unontologies.s3-website-us-east-1.amazonaws.com/undoc#> .
@prefix unvote: <http://unontologies.s3-website-us-east-1.amazonaws.com/unvote#> .
@prefix unorg: <http://unontologies.s3-website-us-east-1.amazonaws.com/unorg#> .
@prefix unsess: <http://unontologies.s3-website-us-east-1.amazonaws.com/unsess#> .
@prefix unagenda: <http://unontologies.s3-website-us-east-1.amazonaws.com/unagenda#> .


# URI for prefix unms will be replaced by something permanently reachable. It will still appear throughout the 
# document in a form that can be globally replaced when the time comes.

unms: a owl:Ontology ;
  dct:title "UN Member States Ontology"@en ;
  dct:contributor "Aaron Helton" ;
  dct:description "An ontology describing current and former UN Member States."@en .

unms:MemberState a rdfs:Class , owl:Class ;
  rdfs:subClassOf skos:Concept ;
  rdfs:label "Member State"@en ;
  rdfs:isDefinedBy <http://unontologies.s3-website-us-east-1.amazonaws.com/unms#> ;
  rdfs:comment "Current UN member state. Labels are of the following types: skos:prefLabel, skos:altLabel, and skos:hiddenLabel."@en .

unms:priorLabel a rdfs:Property , owl:DatatypeProperty ;
  rdfs:subClassOf skos:prefLabel ;
  rdfs:title "Prior Label"@en ;
  rdfs:isDefinedBy <http://unontologies.s3-website-us-east-1.amazonaws.com/unms#> ;
  rdfs:description "Any prior label associated with the MemberState. This should be limited to cases where the name of the country changed but the membership status otherwise stayed the same."@en ;
  skos:example "Belarus changed its name in 1991 from the Byelorussian Soviet Socialist Republic. Thus its entry would have been updated in 1991 such that skos:prefLabel \"Byelorussian Soviet Socialist Republic\"@en would change to skos:prefLabel \"Belarus\"@en, and it would gain unms:priorLabel \"Byelorussian Soviet Socialist Republic\"@en." .

unms:joinDate a rdfs:Property , owl:DatatypeProperty ;
  rdfs:range rdfs:Literal ;
  rdfs:title "Join Date"@en ;
  rdfs:isDefinedBy <http://unontologies.s3-website-us-east-1.amazonaws.com/unms#> ;
  rdfs:description "Date this state was admitted to the UN."@en ;
  rdfs:comment "A member state can have multiple join dates. For instance, Indonesia withdrew on 20 January 1965 and was readmitted on 28 September 1965. Thus it will have two join dates: its original date of 28 September 1950 and its rejoin date of 28 September 1965."@en .

unms:disjoinDate a rdfs:Property , owl:DatatypeProperty ;
  rdfs:range rdfs:Literal ;
  rdfs:title "Disjoin Date"@en ;
  rdfs:isDefinedBy <http://unontologies.s3-website-us-east-1.amazonaws.com/unms#> ;
  rdfs:description "Date this state left the UN, e.g., because of dissolution, withdrawal, etc."@en ;
  rdfs:comment "A member state can have multiple disjoin dates. See the comments for joinDate for an explanation."@en .

unms:isCurrent a rdfs:Property , owl:DatatypeProperty ;
  rdfs:range rdfs:Literal ;
  rdfs:title "Is Current?"@en ;
  rdfs:isDefinedBy <http://unontologies.s3-website-us-east-1.amazonaws.com/unms#> ;
  rdfs:description "Denotes whether this is a current member state; can be inferred from examining joinDate and disjoinDate entries."@en ;
  rdfs:comment "While this could be automatically inferred, such analysis requires close examination of join/withdraw dates. The confounding factor is that each type of date may appear multiple times."@en .

unms:founder a rdfs:Property , owl:DatatypeProperty ;
  rdfs:range rdfs:Literal ;
  rdfs:isDefinedBy <http://unontologies.s3-website-us-east-1.amazonaws.com/unms#> ;
  rdfs:title "Is a founding member"@en ;
  rdfs:description "Denotes whether this member state was a founding member of the UN."@en .

unms:memberThrough a rdfs:Property , owl:ObjectProperty ;
  rdfs:range unms:MemberState ;
  rdfs:title "Denotes that current member inherited membership from a former member, e.g., Russian Federation from USSR."@en ;
  rdfs:description "Represented in the UN as a former member. Ex: ns1:Serbia unms:formerMember ns1:Yugoslavia"@en .
